SeparationLogic/algorithms/Tarjan_directed/Tarjan_scc_basics.v
@@ -29,6 +29,79 @@ Ltac my_destruct H := destruct H as [? [? ?]].
 Tactic Notation "hoare_bind''" uconstr(H) :=
   eapply Hoare_bind; [ | intros; eapply H]; intros.
 
+(** Lifts a pointwise Hoare triple to a general precondition P. *)
+Theorem Hoare_normalize {Σ A: Type}:
+  forall (P: Σ -> Prop) f (Q: A -> Σ -> Prop),
+    (forall s0, P s0 -> Hoare (fun s => s = s0) f Q) ->
+    Hoare P f Q.
+Proof.
+  unfold Hoare. intros.
+  revert H1.
+  apply (H s1); tauto.
+Qed.
+
+(** If P holds at s0, then assume P;; f has the Hoare triple for
+    singleton precondition s = s0. Used for assume-guard elimination. *)
+Theorem Hoare_normal_assume_bind {Σ A: Type}:
+  forall (P: Σ -> Prop) f (Q: A -> Σ -> Prop) s0,
+    (P s0 -> Hoare (fun s => s = s0) f Q) ->
+    (Hoare (fun s => s = s0) (assume P;; f) Q).
+Proof.
+  intros.
+  apply Hoare_assume_bind.
+  apply Hoare_normalize.
+  intros.
+  destruct H0.
+  subst; tauto.
+Qed.
+
+(** Lfix induction principle in normal form: if f W a satisfies Q a s0
+    under the hypothesis that W a does, then Lfix f a also satisfies it. *)
+Theorem Hoare_normal_LFix {Σ A B: Type}:
+  forall (Q: A -> Σ -> B -> Σ -> Prop)
+         (f: (A -> StateRelMonad.M Σ B) -> (A -> StateRelMonad.M Σ B)),
+    (forall (W: A -> StateRelMonad.M Σ B),
+       (forall s0 a, Hoare (fun s => s = s0) (W a) (Q a s0)) ->
+       (forall s0 a, Hoare (fun s => s = s0) (f W a) (Q a s0))) ->
+    (forall s0 a, Hoare (fun s => s = s0) (Lfix f a) (Q a s0)).
+Proof.
+  intros.
+  unfold Hoare.
+  intros s1 b s2 ? ?.
+  change (exists n, (s1, b, s2) ∈ Nat.iter n f ∅ a) in H1.
+  destruct H1 as [n ?].
+  revert s1 b s2 H0 H1.
+  change (Hoare (fun s => s = s0) (Nat.iter n f ∅ a) (Q a s0)).
+  revert s0 a.
+  induction n.
+  + unfold Hoare; simpl; sets_unfold; tauto.
+  + simpl.
+    apply H.
+    apply IHn.
+Qed.
+
+(** Lfix induction with an invariant R closed under the recursive step. *)
+Theorem Hoare_normal_LFix_closed {Σ A B: Type}:
+  forall (R: Σ -> Prop)
+         (Q: A -> Σ -> B -> Σ -> Prop)
+         (f: (A -> StateRelMonad.M Σ B) -> (A -> StateRelMonad.M Σ B)),
+    (forall (W: A -> StateRelMonad.M Σ B),
+       (forall s0 a, R s0 -> Hoare (fun s => s = s0) (W a) (Q a s0)) ->
+       (forall s0 a, R s0 -> Hoare (fun s => s = s0) (f W a) (Q a s0))) ->
+    (forall s0 a, R s0 -> Hoare (fun s => s = s0) (Lfix f a) (Q a s0)).
+Proof.
+  intros R Q f H s0 a HR.
+  unfold Hoare. intros s1 b s2 H0 H1.
+  change (exists n, (s1, b, s2) ∈ Nat.iter n f ∅ a) in H1.
+  destruct H1 as [n ?].
+  revert s1 b s2 H0 H1.
+  change (Hoare (fun s => s = s0) (Nat.iter n f ∅ a) (Q a s0)).
+  revert s0 a HR.
+  induction n.
+  + unfold Hoare; simpl; sets_unfold; tauto.
+  + simpl. apply H. apply IHn.
+Qed.
+
 Section BASICS.
 
   Context {V E: Type}
